Fixed contractiveness of choice

theories/logrel/session_types.v
@@ -18,7 +18,7 @@ Definition lty_message {Σ} (a : action) (M : lmsg Σ) : lsty Σ :=
   Lsty (<a> M).
 
 Definition lty_choice {Σ} (a : action) (Ss : gmap Z (lsty Σ)) : lsty Σ :=
-  Lsty (<a@(x : Z)> MSG #x {{ ⌜is_Some (Ss !! x)⌝ }}; lsty_car (Ss !!! x)).
+  Lsty (<a@(x : Z)> MSG #x {{ ▷ ⌜is_Some (Ss !! x)⌝ }}; lsty_car (Ss !!! x)).
 
 Definition lty_dual {Σ} (S : lsty Σ) : lsty Σ :=
   Lsty (iProto_dual (lsty_car S)).
@@ -83,10 +83,11 @@ Section session_types.
   Proof. solve_proper. Qed.
   Global Instance lty_choice_proper a : Proper ((≡) ==> (≡)) (@lty_choice Σ a).
   Proof. apply ne_proper, _. Qed.
-(* FIXME
   Global Instance lty_choice_contractive a : Contractive (@lty_choice Σ a).
-  Proof. solve_contractive. Qed.
-*)
+  Proof.
+    intros n Ss Ts Heq. rewrite /lty_choice.
+    do 4 f_equiv; f_contractive; [ f_contractive | ]; by rewrite Heq.
+  Qed.
   Global Instance lty_dual_ne : NonExpansive (@lty_dual Σ).
   Proof. solve_proper. Qed.
   Global Instance lty_dual_proper : Proper ((≡) ==> (≡)) (@lty_dual Σ).
